#线性回归
##拟合函数

$\{x_1,x_2,\cdots,x_n\} \mapsto y$，令$x_0=1$
$$
\begin{align}
y &= \sum_{i=1}^n w_ix_i+w_0 \\
&= \sum_{i=0}^n w_ix_i \\
&= x^Tw
\end{align}
$$

##代价函数
###符号定义
$x_{10}=x_{20}=\cdots=x_{m0}=1$

$x_{i*}=\begin{bmatrix}
x_{i0} & x_{i1} & x_{i2} & \cdots & x_{in}
\end{bmatrix}，(i=1,2,\cdots,m)$

$x_{*j}=
\begin{bmatrix}
x_{1j} \\
x_{2j} \\
\vdots \\
x_{mj} \\
\end{bmatrix}，(j=0,1,2,\cdots,n)
$

$Y=
\begin{bmatrix}
y_1 \\
y_2 \\
\vdots \\
y_m
\end{bmatrix}
$

$X=
\begin{bmatrix}
x_{*0} & x_{*1} & x_{*2} & \cdots & x_{*n}
\end{bmatrix}=
\begin{bmatrix}
x_{1*} \\
x_{2*} \\
\vdots \\
x_{m*}
\end{bmatrix}=
\begin{bmatrix}
x_{10} & x_{11} & x_{12} & \cdots & x_{1n} \\
x_{20} & x_{21} & x_{22} & \cdots & x_{2n} \\
\vdots & \vdots & \vdots & \ddots & \vdots \\
x_{m0} & x_{m1} & x_{m2} & \cdots & x_{mn} \\
\end{bmatrix}
$

$w=
\begin{bmatrix}
w_0 \\
w_1 \\
\vdots \\
w_n
\end{bmatrix}
$

###代价函数$J(w)$
$$
J(w_0,w_1,w_2,\cdots,w_n)={1\over 2}\sum_{i=1}^m(y_i-x_{i*}w)^2
$$

##求导解出$w=(X^TX)^{-1}X^TY$
$$
{\partial J \over \partial w_j}=\sum_{i=1}^m -x_{ij}(y_i-x_{i*}w)
= -x_{*j}^T(Y-Xw)
$$

$$
{\partial J \over \partial w}=-X^T(Y-Xw)
$$

令${\partial J \over \partial w}=0$（所有的${\partial J \over w_j}=0，j=0,1,2,\cdots,n $），得
$$ X^T(Y-Xw)=0 \tag{a} $$
$$ w=(X^TX)^{-1}X^TY \tag1 $$


##岭回归
$$ w=\left(X^TX+\lambda I\right)^{-1}X^TY $$

令代价函数
$$
J(w_0,w_1,w_2,\cdots,w_n)={1\over 2}\sum_{i=1}^m(y_i-x_{i*}w)^2+ {1\over 2}\lambda \sum_{j=0}^nw_j^2
$$


$$
{\partial J \over \partial w_j} =
\left( \sum_{i=1}^m -x_{ij}(y_i-x_{i*}w) \right) + w_j
= -x_{*j}^T(Y-Xw) + \lambda w_j
$$

$$
{\partial J \over \partial w}=-X^T(Y-Xw)+\lambda w
$$

令${\partial J \over \partial w}=0$，得
$$ X^T(Y-Xw)=\lambda w=\lambda Iw $$
$$ X^TY=\left(X^TX+\lambda I\right)w $$
$$ w=(X^TX+\lambda I)^{-1}X^TY \tag2 $$


##局部加权
$$ w=\left( X^T WX\right)^{-1}X^TWY $$

$$W=
\begin{bmatrix}
w_{00} & 0 & \cdots & 0 \\
0 & w_{11} & \cdots & 0 \\
\vdots & \vdots & \ddots & \vdots \\
0 & 0 & \cdots & w_{mm} \\
\end{bmatrix}
$$

相当于将$(1)$中的$X^T \mapsto X^TW$

看看推导步骤$(a)$
$$ X^T(Y-Xw)=0 \tag{a} $$

将$X^T \mapsto X^TW$，相当于将m条数据中的每一条乘以一个权重$w_{ii}$

$$ X^TW(Y-Xw)=0 \tag{a} $$













